bag read notation changed

src/LibListZ.v
@@ -13,7 +13,6 @@ Require Export LibBag.
 
 Open Local Scope comp_scope.
 
-
 (* ********************************************************************** *)
 (** * List operations using indices in Z *)
 
@@ -22,8 +21,6 @@ Variables A : Type.
 Implicit Types x : A.
 Implicit Types l : list A.
 Implicit Types i : int.
-
-(** Set up specialized automation for this section *)
 Ltac auto_tilde ::= eauto with maths.
 
 
@@ -32,166 +29,17 @@ Ltac auto_tilde ::= eauto with maths.
 
 (** Functions *)
 
-Definition znth `{Inhab A} (i:int) (l:list A) :=
+Definition length (l:list A) := 
+  (length l) : int.
+
+Definition nth `{Inhab A} (i:int) (l:list A) :=
   If i < 0 then arbitrary else nth (abs i) l. 
 
-Definition zupdate (i:int) (v:A) (l:list A) :=
+Definition update (i:int) (v:A) (l:list A) :=
   If i < 0 then l else LibList.update (abs i) v l.
 
-Definition zmake (n:int) (v:A) :=
+Definition make (n:int) (v:A) :=
   If n < 0 then arbitrary else make (abs n) v.
-
-(** Predicates *)
-
-Definition ZInbound i l := 
-  0 <= i /\ i < length l.
-
-Definition ZNth i l x := 
-  Nth (abs i) l x /\ 0 <= i.
-
-Definition ZUpdate i x l l' :=
-  Update (abs i) x l l' /\ 0 <= i.
-
-
-(* ---------------------------------------------------------------------- *)
-(** * Znth *)
-
-Lemma ZNth_here : forall i x l,
-  i = 0 -> ZNth i (x::l) x.
-Proof using. intros. subst. split~. constructor. Qed. 
-
-Lemma ZNth_zero : forall x l,
-  ZNth 0 (x::l) x.
-Proof using. intros. apply~ ZNth_here. Qed.
-
-Lemma ZNth_next : forall i j x y l,
-  ZNth j l x -> i = j+1 -> ZNth i (y::l) x.
-Proof using.
-  introv [H P] M. subst. split~.
-  applys_eq* Nth_next 3. rew_abs_pos~. 
-Qed.
- 
-Lemma ZNth_app_l : forall i x l1 l2,
-  ZNth i l1 x -> ZNth i (l1 ++ l2) x.
-Proof using. introv [H P]. split~. apply~ Nth_app_l. Qed.
-
-Lemma ZNth_app_r : forall i j x l1 l2,
-  ZNth j l2 x -> i = j + length l1 -> ZNth i (l1 ++ l2) x.
-Proof using.
-  introv [H P]. split~. subst. 
-  apply* Nth_app_r. rew_abs_pos~. 
-Qed.
-
-Lemma ZNth_nil_inv : forall i x,
-  ZNth i nil x -> False.
-Proof using. introv [H P]. apply* Nth_nil_inv. Qed.
-
-Lemma ZNth_cons_inv : forall i x l,
-  ZNth i l x -> 
-     (exists q, l = x::q /\ i = 0)
-  \/ (exists y q j, l = y::q /\ ZNth j q x /\ i = j+1).
-Proof using.
-  introv [H P]. forwards~: (@abs_pos i).
-  destruct (Nth_cons_inv H); unpack.
-  left. exists___. split~. 
-  right. exists___. splits~.
-   split. rewrite* abs_pos_nat. math.
-   math.
-Qed.
-
-Lemma ZNth_inbound : forall i l,
-   ZInbound i l -> exists x, ZNth i l x.
-Proof using.
-  introv [P U]. gen_eq n: (abs i). 
-  gen i l. induction n; intros; 
-    forwards~: (@abs_pos i); destruct l; rew_length in U; try math.
-  math_rewrite (i = 0). exists __. split~. constructor.
-  forwards~ [x [M P']]: (>> IHn (i-1) l).
-    forwards~: (@abs_spos i).
-    exists x. split~. rewrite~ (@abs_spos i). constructor~.
-Qed.
-
-
-(* ---------------------------------------------------------------------- *)
-(** * ZInbound *)
-
-Lemma ZInbound_zero : forall x l,
-  ZInbound 0 (x::l).
-Proof using. split; rew_list~. Qed. 
-
-Lemma ZInbound_zero_not_nil : forall x l,
-  l <> nil -> ZInbound 0 l.
-Proof using. intros. split~. destruct l; tryfalse. rew_list~. Qed.
-
-Lemma ZInbound_cons : forall i j x l,
-  ZInbound j l -> j = i-1 -> ZInbound i (x::l).
-Proof using. introv [P U] H. split; rew_list~. Qed. 
-
-Lemma ZInbound_nil_inv : forall i,
-  ZInbound i nil -> False.
-Proof using. introv [P U]. rew_list in U. math. Qed.
-
-Lemma ZInbound_cons_inv : forall i x l,
-  ZInbound i (x::l) -> i = 0 \/ (i <> 0 /\ ZInbound (i-1) l).
-Proof using.
-  introv [P U]. rew_length in U. tests: (i = 0).
-    left~.
-    right~. split. math. split~.
-Qed.
-
-Lemma ZInbound_cons_pos_inv : forall i x l,
-  ZInbound i (x::l) -> i <> 0 -> ZInbound (i-1) l.
-Proof using.
-  introv H P. destruct* (ZInbound_cons_inv H).
-Qed.
-
-Lemma ZInbound_one_pos_inv : forall i x,
-  ZInbound i (x::nil) -> i <> 0 -> False.
-Proof using.
-  intros. eapply ZInbound_nil_inv. apply* ZInbound_cons_pos_inv.
-Qed.
-
-Lemma ZInbound_app_l_inv : forall i l1 l2,
-  ZInbound i (l1++l2) -> i < length l1 -> ZInbound i l1.
-Proof using. introv [P U] H. split~. Qed. 
-
-Lemma ZInbound_app_r_inv : forall i j l1 l2,
-  ZInbound j (l1++l2) -> j = length l1 + i -> i >= 0 -> ZInbound i l2.
-Proof using. introv [P U] R H. rew_length in U. split~. Qed.
-
-
-(* ---------------------------------------------------------------------- *)
-(** * ZUpdate *)
-
-Lemma ZUpdate_here : forall x y l,
-  ZUpdate 0 x (y::l) (x::l).
-Proof using. split~. apply Update_here. Qed.
-
-Lemma ZUpdate_cons : forall i j x y l l',
-  ZUpdate j x l l' -> i = j+1 -> ZUpdate i x (y::l) (y::l').
-Proof using.
-  introv [U P] H. split~. applys_eq~ Update_cons 4.
-  subst. rew_abs_pos~.
-Qed.  
-
-Lemma ZUpdate_app_l : forall i x l1 l1' l2,
-  ZUpdate i x l1 l1' -> ZUpdate i x (l1++l2) (l1'++l2).
-Proof using. introv [U P]. split~. apply~ Update_app_l. Qed.
-
-Lemma ZUpdate_app_r : forall i j x l1 l2 l2',
-  ZUpdate j x l2 l2' -> i = j + length l1 -> ZUpdate i x (l1++l2) (l1++l2').
-Proof using.
-  introv [U P] H. split~. apply~ Update_app_r. 
-  subst. rew_abs_pos~.
-Qed.
-
-Lemma ZUpdate_not_nil : forall i x l1 l2,
-  ZUpdate i x l1 l2 -> l2 <> nil.
-Proof using. introv [U P]. apply~ Update_not_nil. Qed.
-
-Lemma ZUpdate_length : forall i x l l',
-  ZUpdate i x l l' -> length l = length l'.
-Proof using. introv [U P]. apply~ Update_length. Qed. 
 
 End Zindices.
 
@@ -203,19 +51,18 @@ End Zindices.
     in the specifications. *)
 
 Definition card_impl A (l:list A) : nat :=
-  length l.
+  LibList.length l. 
+  (* todo: should it return a nat or an int? might change... *)
 
 Definition read_impl `{Inhab A} (l:list A) (i:int) : A :=
-  znth i l.
+  nth i l.
 
 Definition update_impl A (l:list A) (i:int) (v:A) : list A :=
-  zupdate i v l.
-
-Definition binds_impl A (l:list A) (i:int) (v:A) : Prop := 
-  ZNth i l v.
+  update i v l.
 
 Definition index_impl A (l:list A) (i:int) : Prop :=
   index (LibList.length l : int) i.
+
 
 Instance card_inst : forall A, BagCard (list A).
  constructor. rapply (@card_impl A). Defined.
@@ -223,13 +70,50 @@ Instance read_inst : forall `{Inhab A}, BagRead int A (list A).
  constructor. rapply (@read_impl A H). Defined.
 Instance update_inst : forall A, BagUpdate int A (list A).
   constructor. rapply (@update_impl A). Defined.
-Instance binds_inst : forall A, BagBinds int A (list A).
-  constructor. rapply (@binds_impl A). Defined.
 Instance index_inst : forall A, BagIndex int (list A).
   constructor. rapply (@index_impl A). Defined.
 
-Global Opaque card_inst read_inst update_inst binds_inst index_inst.
+Global Opaque card_inst read_inst update_inst index_inst.
 
+(* LATER
+Definition binds_impl A (l:list A) (i:int) (v:A) : Prop := 
+  index_impl l i /\ nth i l = v.
+  (* deprecated:  ZNth i l v. *)
+Instance binds_inst : forall A, BagBinds int A (list A).
+  constructor. rapply (@binds_impl A). Defined.
+Global Opaque binds_inst
+*)
+
+(* ---------------------------------------------------------------------- *)
+(** * Properties of length *)
+
+Section LengthProperties.
+Variable A : Type.
+Implicit Types l : list A.
+Ltac auto_tilde ::= eauto with maths.
+
+Lemma length_nil : 
+  length (@nil A) = 0.
+Proof using. auto. Qed.
+Lemma length_cons : forall x l,
+  length (x::l) = 1 + length l.
+Proof using. intros. unfold length. rew_length~. Qed.
+Lemma length_app : forall l1 l2,
+  length (l1 ++ l2) = length l1 + length l2.
+Proof using. intros. unfold length. rew_length~. Qed.
+Lemma length_last : forall x l,
+  length (l & x) = 1 + length l.
+Proof using. intros. unfold length. rew_length~. Qed.
+Lemma length_zero_inv : forall l,
+  length l = 0 -> l = nil.
+Proof using. intros. unfolds length. applys~ LibList.length_zero_inv. Qed.
+
+End LengthProperties.
+
+Hint Rewrite length_nil length_cons length_app
+ length_last length_rev : rew_length.
+Hint Rewrite length_nil length_cons length_app
+ length_last length_rev : rew_list.
 
 
 (* ---------------------------------------------------------------------- *)
@@ -238,20 +122,21 @@ Global Opaque card_inst read_inst update_inst binds_inst index_inst.
 Section MakeProperties.
 Transparent read_inst.
 
-Lemma read_zmake : forall `{Inhab A} (i n:int) (v:A),
-  index n i -> (zmake n v)\(i) = v.
+Lemma read_make : forall `{Inhab A} (i n:int) (v:A),
+  index n i -> (make n v)[i] = v.
 Proof using.
-  introv N. rewrite int_index_def in N. unfold zmake, read_inst, read_impl, znth.
+  introv N. rewrite int_index_def in N. unfold make, read_inst, read_impl, nth.
   case_if. math. simpl. case_if. math.
   applys nth_make. forwards: Zabs_nat_lt i n; try math.
 Qed.
 
-Lemma length_zmake : forall A (n:int) (v:A),
+Lemma length_make : forall A (n:int) (v:A),
   n >= 0 ->
-  length (zmake n v) = n :> int.
+  length (make n v) = n :> int.
 Proof using.
-  introv N. unfold zmake. case_if. math.
-  rewrite length_make. rewrite~ abs_pos.
+  introv N. unfold make. case_if. math.
+  unfold length. rewrite LibList.length_make.
+  rewrite~ abs_pos.
 Qed.
 
 End MakeProperties.
@@ -264,17 +149,17 @@ Section UpdateProperties.
 Transparent index_inst read_inst update_inst.
 
 Lemma length_update : forall A (l:list A) (i:int) (v:A),
-  length (l\(i:=v)) = length l.
+  length (l[i:=v]) = length l.
 Proof using.
-  intros. unfold update_inst, update_impl, zupdate. simpl.
+  intros. unfold update_inst, update_impl, length, update. simpl.
   case_if. math. rewrite~ length_update.
 Qed.
 
 Lemma read_update_case : forall `{Inhab A} (l:list A) (i j:int) (v:A),
-  index l j -> (l\(i:=v))\(j) = (If i = j then v else l\(j)).
+  index l j -> l[i:=v][j] = (If i = j then v else l[j]).
 Proof using.
-  introv. unfold index_inst, index_impl, update_inst, update_impl, zupdate,
-    read_inst, read_impl, znth. simpl. introv N. rewrite int_index_def in N.
+  introv. unfold index_inst, index_impl, update_inst, update_impl, update,
+    read_inst, read_impl, nth. simpl. introv N. rewrite int_index_def in N.
   case_if. math.
   case_if. case_if. auto. case_if. 
     rewrite~ nth_update_eq. apply nat_int_lt. rewrite abs_pos; try math.
@@ -283,12 +168,12 @@ Proof using.
 Qed.
 
 Lemma read_update_eq : forall `{Inhab A} (l:list A) (i:int) (v:A),
-  index l i -> (l\(i:=v))\(i) = v.
+  index l i -> (l[i:=v])[i] = v.
 Proof using. introv N. rewrite~ read_update_case. case_if~. Qed.
 
 Lemma read_update_neq : forall `{Inhab A} (l:list A) (i j:int) (v:A),
-  index l j -> (i <> j) -> (l\(i:=v))\(j) = l\(j).
-Proof using. introv N. rewrite~ read_update_case. case_if~. Qed.
+  index l j -> (i <> j) -> (l[i:=v])[j] = l[j].
+Proof using. introv N. rewrite~ read_update_case. case_if; auto_false~. Qed.
 
 End UpdateProperties.
 
@@ -299,7 +184,7 @@ End UpdateProperties.
 (** [rew_arr] is a light normalization tactic for array *)
 
 (* TODO: rename to [rew_array_nocase] *) 
-Hint Rewrite @read_zmake @length_zmake @length_update @read_update_eq 
+Hint Rewrite @read_make @length_make @length_update @read_update_eq 
   : rew_arr.
 
 Tactic Notation "rew_arr" := 
@@ -325,7 +210,7 @@ Tactic Notation "rew_arr" "*" "in" "*" :=
 
 (** [rew_array] is a normalization tactic for array *)
 
-Hint Rewrite @read_zmake @length_zmake @length_update @read_update_eq
+Hint Rewrite @read_make @length_make @length_update @read_update_eq
   @read_update_case : rew_array.
 
 Tactic Notation "rew_array" := 
@@ -376,14 +261,14 @@ Lemma index_bounds_impl : forall A (l:list A) i,
 Proof using. intros. rewrite~ index_bounds. Qed.
 
 Lemma index_update : forall A (l:list A) i j (v:A),
-  index l i -> index (l\(j:=v)) i.
+  index l i -> index (l[j:=v]) i.
 Proof using. intros. rewrite index_def in *. rewrite~ length_update. Qed.
 
 Lemma index_zmake : forall A n i (v:A),
-  index n i -> index (zmake n v) i.
+  index n i -> index (make n v) i.
 Proof using.
   introv H. rewrite index_def. rewrite int_index_def in H.
-  rewrite~ length_zmake. math.
+  rewrite~ length_make. math.
 Qed.
 
 End IndexProperties.
@@ -398,34 +283,34 @@ Require Import LibWf.
 
 (* TODO: implement a non-decidable version of count *)
 
-Parameter zcount : forall A (P:A->Prop) (l:list A), int.
+Parameter count : forall A (P:A->Prop) (l:list A), int.
 
 (* currently not used
 Parameter count_make : forall A (f:A->Prop) n v,
   count f (make n v) = (If f v then n else 0).
 *)
 
-Parameter zcount_update : forall `{Inhab A} (P:A->Prop) (l:list A) (i:int) v,
+Parameter count_update : forall `{Inhab A} (P:A->Prop) (l:list A) (i:int) v,
   index l i ->
-  zcount P (l\(i:=v)) = zcount P l
-    - (If P (l\(i)) then 1 else 0)
+  count P (l[i:=v]) = count P l
+    - (If P (l[i]) then 1 else 0)
     + (If P v then 1 else 0).
 
-Parameter zcount_bounds : forall `{Inhab A} (l:list A) (P:A->Prop),
-  0 <= zcount P l <= length l.
+Parameter count_bounds : forall `{Inhab A} (l:list A) (P:A->Prop),
+  0 <= count P l <= length l.
 
 (** The following lemma is used to argue that the update to a sequence,
     when writing a value that satisfies [P] in place of one that did not
     satisfy [P], decreases the total number of values that satisfying 
     [P] in the sequence. *)
 
-Lemma zcount_upto : forall `{Inhab A} (P:A->Prop) (l:list A) (n i:int) (v:A),
-  ~ P (l\(i)) -> P v -> index l i -> (length l <= n)%Z ->
-  upto n (zcount P (l\(i:=v))) (zcount P l).
+Lemma count_upto : forall `{Inhab A} (P:A->Prop) (l:list A) (n i:int) (v:A),
+  ~ P (l[i]) -> P v -> index l i -> (length l <= n)%Z ->
+  upto n (count P (l[i:=v])) (count P l).
 Proof using.
-  introv Ni Pv Hi Le. forwards K: (zcount_bounds (l\(i:=v)) P). split.
+  introv Ni Pv Hi Le. forwards K: (count_bounds (l[i:=v]) P). split.
   rewrite length_update in K. math.
-  lets M: (@zcount_update A _). rewrite~ M. clear M. 
+  lets M: (@count_update A _). rewrite~ M. clear M. 
   do 2 (case_if; tryfalse). math.
 Qed.
 
@@ -440,3 +325,181 @@ Lemma isTrue_eq_list : forall A {IA:Inhab A} (L1 L2:list A),
   (L1 = L2)).
 
 *)
+
+
+
+
+
+(* ********************************************************************** *)
+(** * DEPRECATED -- List predicates using indices in Z *)
+
+Section ZindicesOld.
+Variables A : Type.
+Implicit Types x : A.
+Implicit Types l : list A.
+Implicit Types i : int.
+Ltac auto_tilde ::= eauto with maths.
+
+(* ---------------------------------------------------------------------- *)
+(** * DEPRECATED *)
+
+(** Predicates *)
+
+Definition ZInbound i l := 
+  0 <= i /\ i < length l.
+
+Definition ZNth i l x := 
+  Nth (abs i) l x /\ 0 <= i.
+
+Definition ZUpdate i x l l' :=
+  Update (abs i) x l l' /\ 0 <= i.
+
+
+(* ---------------------------------------------------------------------- *)
+(** * DEPRECATED -- Znth *)
+
+Lemma ZNth_here : forall i x l,
+  i = 0 -> ZNth i (x::l) x.
+Proof using. intros. subst. split~. constructor. Qed. 
+
+Lemma ZNth_zero : forall x l,
+  ZNth 0 (x::l) x.
+Proof using. intros. apply~ ZNth_here. Qed.
+
+Lemma ZNth_next : forall i j x y l,
+  ZNth j l x -> i = j+1 -> ZNth i (y::l) x.
+Proof using.
+  introv [H P] M. subst. split~.
+  applys_eq* Nth_next 3. rew_abs_pos~. 
+Qed.
+ 
+Lemma ZNth_app_l : forall i x l1 l2,
+  ZNth i l1 x -> ZNth i (l1 ++ l2) x.
+Proof using. introv [H P]. split~. apply~ Nth_app_l. Qed.
+
+Lemma ZNth_app_r : forall i j x l1 l2,
+  ZNth j l2 x -> i = j + length l1 -> ZNth i (l1 ++ l2) x.
+Proof using.
+  introv [H P]. unfold length. split~. subst. 
+  apply* Nth_app_r. rew_abs_pos~. 
+Qed.
+
+Lemma ZNth_nil_inv : forall i x,
+  ZNth i nil x -> False.
+Proof using. introv [H P]. apply* Nth_nil_inv. Qed.
+
+Lemma ZNth_cons_inv : forall i x l,
+  ZNth i l x -> 
+     (exists q, l = x::q /\ i = 0)
+  \/ (exists y q j, l = y::q /\ ZNth j q x /\ i = j+1).
+Proof using.
+  introv [H P]. forwards~: (@abs_pos i).
+  destruct (Nth_cons_inv H); unpack.
+  left. exists___. split~. 
+  right. exists___. splits~.
+   split. rewrite* abs_pos_nat. math.
+   math.
+Qed.
+
+Lemma ZNth_inbound : forall i l,
+   ZInbound i l -> exists x, ZNth i l x.
+Proof using.
+  introv [P U]. unfolds length. gen_eq n: (abs i). 
+  gen i l. induction n; intros; 
+    forwards~: (@abs_pos i); destruct l; rew_length in U; try math.
+  math_rewrite (i = 0). exists __. split~. constructor.
+  forwards~ [x [M P']]: (>> IHn (i-1) l).
+    forwards~: (@abs_spos i).
+    exists x. split~. rewrite~ (@abs_spos i). constructor~.
+Qed.
+
+
+(* ---------------------------------------------------------------------- *)
+(** * DEPRECATED -- ZInbound *)
+
+Lemma ZInbound_zero : forall x l,
+  ZInbound 0 (x::l).
+Proof using. split; unfold length; rew_list~. Qed. 
+
+Lemma ZInbound_zero_not_nil : forall x l,
+  l <> nil -> ZInbound 0 l.
+Proof using.
+  intros. split~. unfold length.
+  destruct l; tryfalse. rew_list~. 
+Qed.
+
+Lemma ZInbound_cons : forall i j x l,
+  ZInbound j l -> j = i-1 -> ZInbound i (x::l).
+Proof using. introv [P U] H. split; rew_list~. Qed. 
+
+Lemma ZInbound_nil_inv : forall i,
+  ZInbound i nil -> False.
+Proof using. introv [P U]. rew_list in U. math. Qed.
+
+Lemma ZInbound_cons_inv : forall i x l,
+  ZInbound i (x::l) -> i = 0 \/ (i <> 0 /\ ZInbound (i-1) l).
+Proof using.
+  introv [P U]. rew_length in U. tests: (i = 0).
+    left~.
+    right~. split. math. split~.
+Qed.
+
+Lemma ZInbound_cons_pos_inv : forall i x l,
+  ZInbound i (x::l) -> i <> 0 -> ZInbound (i-1) l.
+Proof using.
+  introv H P. destruct* (ZInbound_cons_inv H).
+Qed.
+
+Lemma ZInbound_one_pos_inv : forall i x,
+  ZInbound i (x::nil) -> i <> 0 -> False.
+Proof using.
+  intros. eapply ZInbound_nil_inv. apply* ZInbound_cons_pos_inv.
+Qed.
+
+Lemma ZInbound_app_l_inv : forall i l1 l2,
+  ZInbound i (l1++l2) -> i < length l1 -> ZInbound i l1.
+Proof using. introv [P U] H. split~. Qed. 
+
+Lemma ZInbound_app_r_inv : forall i j l1 l2,
+  ZInbound j (l1++l2) -> j = length l1 + i -> i >= 0 -> ZInbound i l2.
+Proof using. introv [P U] R H. rew_length in U. split~. Qed.
+
+
+(* ---------------------------------------------------------------------- *)
+(** * DEPRECATED -- ZUpdate *)
+
+Lemma ZUpdate_here : forall x y l,
+  ZUpdate 0 x (y::l) (x::l).
+Proof using. split~. apply Update_here. Qed.
+
+Lemma ZUpdate_cons : forall i j x y l l',
+  ZUpdate j x l l' -> i = j+1 -> ZUpdate i x (y::l) (y::l').
+Proof using.
+  introv [U P] H. split~. applys_eq~ Update_cons 4.
+  subst. rew_abs_pos~.
+Qed.  
+
+Lemma ZUpdate_app_l : forall i x l1 l1' l2,
+  ZUpdate i x l1 l1' -> ZUpdate i x (l1++l2) (l1'++l2).
+Proof using. introv [U P]. split~. apply~ Update_app_l. Qed.
+
+Lemma ZUpdate_app_r : forall i j x l1 l2 l2',
+  ZUpdate j x l2 l2' -> i = j + length l1 -> ZUpdate i x (l1++l2) (l1++l2').
+Proof using.
+  introv [U P] H. unfolds length. split~. apply~ Update_app_r. 
+  subst. rew_abs_pos~.
+Qed.
+
+Lemma ZUpdate_not_nil : forall i x l1 l2,
+  ZUpdate i x l1 l2 -> l2 <> nil.
+Proof using. introv [U P]. apply~ Update_not_nil. Qed.
+
+Lemma ZUpdate_length : forall i x l l',
+  ZUpdate i x l l' -> length l = length l'.
+Proof using.
+  introv [U P]. unfolds length.
+  forwards~: Update_length. 
+Qed. 
+
+
+End ZindicesOld.
