src/LibReflect.v
@@ -8,6 +8,8 @@ Require Import LibTactics.
 Require Export LibBool LibLogic.
 Generalizable Variable P.
 
+
+
 (* ********************************************************************** *)
 (** * Reflection between booleans and propositions *)
 
